Switch to using evaluation contexts

src/Ctxt.v
@@ -20,50 +20,179 @@ Context `{HostExprs A}.
 
 Open Scope Ty_scope.
 
-Inductive Ctxt Γ : Ty → Type :=
-  | C_Hole {τ} : Ctxt Γ τ
+(* A context defines a hole which, after substitution, yields an expression of
+   the index type. *)
+Inductive Ctxt Γ τ' : Ty → Type :=
+  | C_Hole : Ctxt Γ τ' τ'
 
-  (* | C_If1 {τ} : Ctxt Γ TyBool → Exp Γ τ → Exp Γ τ → Ctxt Γ TyBool *)
+  (* | C_If1 {τ} : Ctxt Γ τ' TyBool → Exp Γ τ → Exp Γ τ → Ctxt Γ τ' TyBool *)
   (* | C_If2 {τ} : Exp Γ TyBool → Ctxt Γ τ → Exp Γ τ → Ctxt Γ τ *)
   (* | C_If3 {τ} : Exp Γ TyBool → Exp Γ τ → Ctxt Γ τ → Ctxt Γ τ *)
 
-  | C_App1 {dom cod} : Ctxt Γ (dom ⟶ cod) -> Exp Γ dom -> Ctxt Γ (dom ⟶ cod)
-  | C_App2 {dom cod} : Exp Γ (dom ⟶ cod) -> Ctxt Γ dom -> Ctxt Γ dom.
+  | C_App1 {dom cod} : Ctxt Γ τ' (dom ⟶ cod) → Exp Γ dom → Ctxt Γ τ' cod
+  | C_App2 {dom cod} : Exp Γ (dom ⟶ cod) → Ctxt Γ τ' dom → Ctxt Γ τ' cod.
 
-Derive Signature NoConfusion NoConfusionHom for Ctxt.
+Derive Signature NoConfusion for Ctxt.
 
-Inductive Plug : ∀ {Γ τ τ'}, Ctxt Γ τ → Exp Γ τ → Exp Γ τ' → Prop :=
-  | Plug_Hole {Γ τ} (e : Exp Γ τ) : Plug (C_Hole _) e e
+(*
+Equations Plug {Γ τ' τ} (e : Exp Γ τ') (c : Ctxt Γ τ' τ) : Exp Γ τ :=
+  Plug e (C_Hole _ _)      := e;
+  Plug e (C_App1 _ _ C e1) := APP (Plug e C) e1;
+  Plug e (C_App2 _ _ e1 C) := APP e1 (Plug e C).
+*)
+
+Inductive Plug {Γ τ'} : ∀ {τ}, Exp Γ τ' → Ctxt Γ τ' τ → Exp Γ τ → Prop :=
+  | Plug_Hole (e : Exp Γ τ') : Plug e (C_Hole _ _) e
 
   (* | Plug_If1 {Γ τ} (C : Ctxt Γ TyBool) (e e' : Exp Γ TyBool) (e1 e2 : Exp Γ τ) : *)
-  (*   Plug C e e' -> Plug (C_If1 _ C e1 e2) e (If e' e1 e2) *)
+  (*   Plug C e e' → Plug (C_If1 _ C e1 e2) e (If e' e1 e2) *)
   (* | Plug_If2 {Γ τ} (C : Ctxt Γ τ) (e e' : Exp Γ τ) e1 (e2 : Exp Γ τ) : *)
-  (*   Plug C e e' -> Plug (C_If2 _ e1 C e2) e (If e1 e' e2) *)
+  (*   Plug C e e' → Plug (C_If2 _ e1 C e2) e (If e1 e' e2) *)
   (* | Plug_If3 {Γ τ} (C : Ctxt Γ τ) (e e' : Exp Γ τ) e1 (e2 : Exp Γ τ) : *)
-  (*   Plug C e e' -> Plug (C_If3 _ e1 e2 C) e (If e1 e2 e') *)
+  (*   Plug C e e' → Plug (C_If3 _ e1 e2 C) e (If e1 e2 e') *)
 
-  | Plug_App1 {Γ dom cod} (C : Ctxt Γ (dom ⟶ cod)) (e e' : Exp Γ (dom ⟶ cod))
-              (e1 : Exp Γ dom) :
-    Plug C e e' -> Plug (C_App1 _ C e1) e (APP e' e1)
-  | Plug_App2 {Γ dom cod} (C : Ctxt Γ dom) (e e' : Exp Γ dom)
-              (e1 : Exp Γ (dom ⟶ cod)) :
-    Plug C e e' -> Plug (C_App2 _ e1 C) e (APP e1 e').
+  | Plug_App1 {dom cod} {C : Ctxt Γ τ' (dom ⟶ cod)}
+              {e : Exp Γ τ'} {e' : Exp Γ (dom ⟶ cod)}
+              {e1 : Exp Γ dom} :
+    Plug e C e' →
+    Plug e (C_App1 _ _ C e1) (APP e' e1)
+  | Plug_App2 {dom cod} {C : Ctxt Γ τ' dom}
+              {e : Exp Γ τ'} {e' : Exp Γ dom}
+              {e1 : Exp Γ (dom ⟶ cod)} :
+    ValueP e1 →
+    Plug e C e' →
+    Plug e (C_App2 _ _ e1 C) (APP e1 e').
 
 Derive Signature for Plug.
 
-Inductive Step0 : ∀ {Γ τ}, Exp Γ τ -> Exp Γ τ -> Prop :=
-  | ST_AppAbs0 {Γ dom cod} (e : Exp (dom :: Γ) cod) v :
-    ValueP v -> Step0 (APP (LAM e) v) (SubExp {|| v ||} e).
+Inductive Redex {Γ} : ∀ {τ}, Exp Γ τ → Exp Γ τ → Prop :=
+  | ST_AppAbs0 {dom cod} (e : Exp (dom :: Γ) cod) v :
+    ValueP v →
+    Redex (APP (LAM e) v) (SubExp {|| v ||} e).
 
-Derive Signature for Step0.
+Derive Signature for Redex.
 
-Inductive Step : ∀ {Γ τ}, Exp Γ τ -> Exp Γ τ -> Prop :=
-  | StepRule {Γ τ} (C : Ctxt Γ τ) (e1 e1' e2 e2' : Exp Γ τ) :
-    Plug C e1 e1' ->
-    Plug C e2 e2' ->
-    Step0 e1 e2 ->
-    Step e1' e2'.
+Reserved Notation " t '--->' t' " (at level 40).
+
+Inductive Step : ∀ {Γ τ}, Exp Γ τ → Exp Γ τ → Prop :=
+  | StepRule {Γ τ' τ} {C : Ctxt Γ τ' τ}
+             {e1 e2 : Exp Γ τ'} {e1' e2' : Exp Γ τ} :
+    Plug e1 C e1' →
+    Plug e2 C e2' →
+    Redex e1 e2 →
+    e1' ---> e2'
+
+  where " t '--->' t' " := (Step t t').
 
 Derive Signature for Step.
 
+#[local] Hint Constructors ValueP Plug Redex Step : core.
+
+Theorem strong_progress {τ} (e : Exp [] τ) :
+  ValueP e ∨ ∃ e', e ---> e'.
+Proof.
+  dependent induction e; reduce.
+  - now inv v.
+  - now left; constructor.
+  - right.
+    destruct IHe1 as [V1|[e1' H1']];
+    destruct IHe2 as [V2|[e2' H2']].
+    + dependent elimination V1.
+      now eauto 6.
+    + dependent elimination H2'.
+      now eauto 6.
+    + dependent elimination H1'.
+      now eauto 6.
+    + dependent elimination H1'.
+      dependent elimination H2'.
+      now eauto 6.
+Qed.
+
+Lemma Plug_not_ValueP {Γ τ} {C : Ctxt Γ τ τ} (e v : Exp Γ τ) :
+  ValueP v →
+  Plug e C v →
+    C = C_Hole _ _ ∧ e = v.
+Proof.
+  intros.
+  dependent elimination H0.
+  now inv H1.
+Qed.
+
+Lemma Redex_ValueP {Γ τ} (e v : Exp Γ τ) :
+  ValueP v →
+    ¬ Redex v e.
+Proof.
+  repeat intro.
+  dependent elimination H0.
+  now inv H1.
+Qed.
+
+Lemma Plug_deterministic {Γ τ τ'} {C : Ctxt Γ τ' τ} e2 :
+  ∀ e1 e1', Redex e1 e1' →
+  ∀ τ'' f1 f1', Redex f1 f1' →
+  Plug e1 C e2 →
+    ∀ (C' : Ctxt Γ τ'' τ),
+      Plug f1 C' e2 →
+      τ' = τ'' ∧ C ~= C' ∧ e1 ~= f1.
+Proof.
+  intros.
+  generalize dependent C'.
+  induction H2; intros; subst.
+  inv H3; auto.
+  - exfalso.
+    dependent elimination H0.
+    dependent elimination H1.
+    now inv H7.
+  - exfalso.
+    dependent elimination H0.
+    dependent elimination H1.
+    now inv H8.
+  - dependent elimination H3.
+    + exfalso.
+      dependent elimination H0.
+      dependent elimination H1.
+      now inv H2.
+    + intuition.
+      now destruct (H3 _ p); reduce.
+    + exfalso.
+      dependent elimination H0.
+      dependent elimination H1.
+      now inv H2.
+  - dependent elimination H4.
+    + exfalso.
+      dependent elimination H0.
+      dependent elimination H1.
+      now inv H3.
+    + exfalso.
+      dependent elimination H0.
+      dependent elimination H1.
+      now inv p.
+    + intuition.
+      now destruct (H4 _ p0); reduce.
+Qed.
+
+Lemma Plug_functional {Γ τ τ'} {C : Ctxt Γ τ' τ} e e1 :
+  Plug e C e1
+    → ∀ e2, Plug e C e2 → e1 = e2.
+Proof.
+  intros.
+  dependent induction H0.
+  - now inv H1.
+  - dependent destruction H1.
+    now f_equal; auto.
+  - dependent destruction H2.
+    now f_equal; auto.
+Qed.
+
+Lemma Redex_deterministic : ∀ Γ τ (e e' : Exp Γ τ),
+  Redex e e' → ∀ e'', Redex e e'' → e' = e''.
+Proof.
+  intros.
+  dependent elimination H0.
+  dependent elimination H1.
+  reflexivity.
+Qed.
+
 End Ctxt.
+
+Notation " t '--->' t' " := (Step t t') (at level 40).
